Cleaned executable code; updated doc; added forgotten commits

ML/Muntax.sml
@@ -56,4 +56,109 @@ fun check_and_verify_from_stream stream _ =
     else input ^ " " |> run_and_print check_deadlock
   end;
 
-val main = check_and_verify_from_stream TextIO.stdIn
+fun find_with_arg P [] = NONE
+  | find_with_arg P [_] = NONE
+  | find_with_arg P (x :: y :: xs) = if P x then SOME y else find_with_arg P (y :: xs)
+
+fun read_file f =
+  let
+    val file = TextIO.openIn f
+    val s = read_lines file
+    val _ = TextIO.closeIn file
+  in s end;
+
+val to_large_int = fn x => x;
+
+fun print_usage () =
+  let
+    val prelude = "Usage:\n"
+    val usage = [
+      ("m ", "Input file for the model & formula. "
+          ^ "If this is not specified, the input is read from stdin."),
+      ("dc", "Ignore formula and run deadlock check."),
+      ("e ", "Report set of explored states (only works for reachability formulas)."),
+      ("s ", "Print back the JSON that was parsed from the input.")
+    ]
+  in
+    usage
+    |> map (fn (opt, s) => "-" ^ opt ^ ": " ^ s ^ "\n")
+    |> String.concat
+    |> (fn s => prelude ^ s)
+    |> println
+ end
+
+fun print_explored () =
+  let
+    val messages = Logging.get_trace ()
+    val explored = filter (fn (i, s) => i = 5 andalso String.isPrefix "Explored: " s) messages
+    val explored = map (fn (_, s) => String.extract (s, String.size "Explored: ", NONE)) explored
+    val final = filter (fn (i, s) => i = 5 andalso String.isPrefix "Final: " s) messages
+    val final = map (fn (_, s) => String.extract (s, String.size "Final: ", NONE)) final
+    val _ = println ""
+    val _ = println "The search explored the following states:"
+    val _ = map println explored
+    val _ = if length final > 0 then println "The search hit the following final state:" else ()
+    val _ = if length final > 0 then map println final else [()]
+  in () end
+
+fun print_json () =
+  let
+    val messages = Logging.get_trace ()
+    val jsons = filter (fn (i, s) => i = 2) messages |> map snd
+    val _ = println ""
+    val _ = println "The following JSON was read by the parser:"
+    val _ = if length jsons > 0 then println (hd jsons) else ()
+  in () end
+
+fun main () =
+  let
+    val args = CommandLine.arguments()
+    val check_deadlock = List.find (fn x => x = "-deadlock" orelse x = "-dc") args <> NONE
+    val cpu_time = List.find (fn x => x = "-cpu-time" orelse x = "-cpu") args <> NONE
+    val trace_explored = List.find (fn x => x = "-explored" orelse x = "-e") args <> NONE
+    val model = find_with_arg (fn x => x = "-model" orelse x = "-m") args
+    val num_threads = find_with_arg (fn x => x = "-num-threads" orelse x = "-n") args
+    val show_json = List.find (fn x => x = "-show" orelse x = "-s") args <> NONE
+    val show_help = List.find (fn x => x = "-help" orelse x = "-h" orelse x = "-?") args <> NONE
+    fun convert f NONE = NONE
+      | convert f (SOME x) = SOME (f x)
+        handle Fail msg => (println ("Argument error: " ^ msg); OS.Process.exit OS.Process.failure)
+    fun int_of_string err_msg s = case Int.fromString s of
+        NONE => raise Fail (err_msg ^ " should be an integer")
+      | SOME x => x
+    fun the_default x NONE = x
+      | the_default _ (SOME x) = x
+    val num_threads = num_threads
+      |> convert (int_of_string "Number of threads")
+      |> the_default 1
+    val _ = println "** Configuration options **"
+    val _ = "* Deadlock: " ^ (if check_deadlock then "True" else "False") |> println
+    val _ = "* Model: " ^ (case model of NONE => "from stdin" | SOME m => m) |> println
+    val _ = "* Report explored states: " ^ (if trace_explored then "True" else "False") |> println
+    (* val _ = "* Num Threads: " ^ Int.toString num_threads |> println *)
+    (* val _ = "* Measuring CPU time: " ^ (if cpu_time then "True" else "False") |> println *)
+    val num_threads = 10000
+    (* val num_threads = num_threads |> to_large_int |> nat_of_integer *)
+    (* val _ = if cpu_time then Timing.set_cpu true else () *)
+    val _ = if show_json then Logging.set_level 2 else ()
+    val _ = if trace_explored then Logging.set_level 5 else ()
+    val input = ref ""
+  in
+    if show_help then
+      print_usage ()
+    else (case model of
+      NONE => input := read_lines TextIO.stdIn |
+      SOME f =>
+        let
+          val file = TextIO.openIn f
+          val s = read_lines file
+          val _ = TextIO.closeIn file
+          val _ = input := s
+        in () end;
+      run_and_print check_deadlock (!input);
+      (if show_json then print_json () else ());
+      (if trace_explored then print_explored () else ())
+    )
+  end
+
+(* val main = check_and_verify_from_stream TextIO.stdIn *)
