README.md
@@ -27,20 +27,15 @@ cd ML
 make
 ```
 
-#### To build the checker with OCaml:
-Replace `Big_int` with `Big_int_Z` in `UPPAAL_Model_Checker.ml` and `to_int` with `int_of_big_int`.
-Then run
-```
-cd ML
-ocamlfind ocamlopt -package zarith -package angstrom -linkpkg nums.cmxa -linkpkg UPPAAL_Model_Checker.ml -linkpkg Checker.ml
-```
-
 #### To browse the sources interactively in Isabelle:
 Install [Isabelle](https://isabelle.in.tum.de/) and the [AFP](https://www.isa-afp.org/using.shtml). Then run:
 ```
 isabelle jedit -l Refine_Imperative_HOL
 ```
 and open one of the `.thy` files.
+A good starting point is the file where the model checker is exported to executable code:
+`Simple_Networks/Simple_Network_Language_Export_Code.thy`.
+
 
 #### To build the Isabelle sources and extract the checker source code:
 Install [Isabelle](https://isabelle.in.tum.de/) and the [AFP](https://www.isa-afp.org/using.shtml). Then run:
@@ -58,18 +53,45 @@ python server.py
 The server will run under port 3069 and communicates with the GUI.
 
 ## Running
-Pick one of the files from `benchmarks` and run:
+Pick one of the `.muntax` files from `benchmarks` and run:
 ```
-ML/munta < benchmarks/<the_benchmark>.munta
+ML/munta -m benchmarks/<the_benchmark>.muntax
+```
+To list MUNTA's command line options, run:
+```
+ML/munta -h
 ```
 
 ## Documentation
+
+### Input Format
+MUNTA accepts a simple modeling language, which is formally described in the file
+`Simple_Networks/Simple_Network_Language.thy`.
+Input models and formulas are specified in the JSON format (MUNTA's file ending: `.muntax`).
+Examples can be found in the folder `benchmarks`.
+
+## Benchmarks
+The benchmarks are derived from the [UPPAAL](https://www.it.uu.se/research/group/darts/uppaal/benchmarks/) and
+[TChecker](http://www.labri.fr/perso/herbrete/tchecker/) benchmarks.
+
+
+
+## Outdated
+The following instructions are outdated and in the progress of being updated:
 
 ### Input Format
 MUNTA is aimed at understanding bytecode produced by [UPPAAL](http://uppaal.org/).
 However, for the time being, this bytecode needs to be pre-processed slightly.
 You can find some pre-processed benchmarks in `benchmarks`.
 The input format is documented in `UPPAAL_Asm.thy` and `ML/Checker.sml`.
+
+#### To build the checker with OCaml:
+Replace `Big_int` with `Big_int_Z` in `UPPAAL_Model_Checker.ml` and `to_int` with `int_of_big_int`.
+Then run
+```
+cd ML
+ocamlfind ocamlopt -package zarith -package angstrom -linkpkg nums.cmxa -linkpkg UPPAAL_Model_Checker.ml -linkpkg Checker.ml
+```
 
 ### Isabelle Formalizations
 Human readable `.pdf` documents (with textual annotations) of the formalizations can be produced by Isabelle.
@@ -82,7 +104,3 @@ and you will get the following:
 - `output/abstract_reachability.pdf`: the abstract formalization of reachability checking for Timed Automata
 - `output/model_checking.pdf`: the formalization of MUNTA and the route from the abstract formalization to the correctness proof for MUNTA
 - `output/abstract_reachability_proofs.pdf`, `output/model_checking_proofs.pdf`: variants of the above documents with proofs
-
-## Benchmarks
-The benchmarks are derived from the [UPPAAL](https://www.it.uu.se/research/group/darts/uppaal/benchmarks/) and
-[TChecker](http://www.labri.fr/perso/herbrete/tchecker/) benchmarks.
